First half lemmas done for parching the juicy machine (Erasure, instantiated for Clight).

concurrency/Clight_erasure.v
@@ -2,10 +2,18 @@ Add LoadPath "../concurrency" as concurrency.
 
 Require Import compcert.common.Memory.
 
+
+Require Import veric.compcert_rmaps.
+Require Import veric.juicy_mem.
+Require Import veric.res_predicates.
+
+(*IM using proof irrelevance!*)
+Require Import ProofIrrelevance.
+
 (* The concurrent machinery*)
 Require Import concurrency.concurrent_machine.
 Require Import concurrency.juicy_machine. Import Concur.
-Require Import concurrency.compcert_threads. Import Concur.
+Require Import concurrency.dry_machine. Import Concur.
 
 (*The simulations*)
 Require Import sepcomp.wholeprog_simulations.
@@ -13,21 +21,162 @@ Require Import sepcomp.wholeprog_simulations.
 (*General erasure*)
 Require Import concurrency.erasure.
 
-Module ClightErasure (SCH: Scheduler NatTID)(SEM: Semantics)<:Parching SCH SEM.
-  Import SEM.
-  Import juicy_machine.
-  Import compcert_threads.
-  
-  Module JSEM:= JuicyMachineSig SEM.
-  Module JuicyMachine:= CoarseMachine NatTID SCH JSEM.
-  Definition JMachineSem:= JuicyMachine.MachineSemantics.
-  Notation jstate:= JSEM.machine_state.
-  
-  Module DSEM:= ShareMachineSig SEM.
-  Module DryMachine:= CoarseMachine NatTID SCH DSEM.
-  Definition DMachineSem:= DryMachine.MachineSemantics.
-  Notation dstate:= DSEM.machine_state.
+(* I will import this from CLight once we port it*)
+(*Module ClightSEM<: Semantics.
+  Definition G:= nat.
+  Definition C:= nat.
+  Definition M:= Mem.mem.
+  Definition  
+End ClightSEM.*)
 
+Module ClightParching <: ErasureSig.
+
+  Declare Module ClightSEM: Semantics. (*This will be imported from Clight wonce we port it*)
+  Module SCH:= ListScheduler NatTID.            
+  Module SEM:= ClightSEM.
+  Import SCH SEM.
+
+  Module JSEM:= JuicyMachineShell SEM .
+  Module JuicyMachine:= CoarseMachine SCH JSEM.
+  Notation JMachineSem:= JuicyMachine.MachineSemantics.
+  Notation jstate:= JuicyMachine.SIG.ThreadPool.t.
+  Notation jmachine_state:= JuicyMachine.MachState.
+  Module JTP:=JuicyMachine.SIG.ThreadPool.
+  
+  Module DSEM:= DryMachineShell SEM.
+  Module DryMachine:= CoarseMachine SCH DSEM.
+  Notation DMachineSem:= DryMachine.MachineSemantics. 
+  Notation dstate:= DryMachine.SIG.ThreadPool.t.
+  Notation dmachine_state:= DryMachine.MachState.
+  Module DTP:=DryMachine.SIG.ThreadPool.
+
+  (*Parameter parch_state : jstate ->  dstate.*)
+  Inductive match_st : jstate ->  dstate -> Prop:=
+    MATCH_ST: forall (js:jstate) ds
+                (mtch_cnt: forall {tid},  JTP.containsThread js tid -> DTP.containsThread ds tid )
+                (mtch_cnt': forall {tid}, DTP.containsThread ds tid -> JTP.containsThread js tid )
+                (mtch_gtc: forall {tid} (Htid:JTP.containsThread js tid), JTP.getThreadC Htid = DTP.getThreadC (mtch_cnt Htid) )
+                (mtch_perm: forall b ofs {tid} (Htid:JTP.containsThread js tid),
+                    juicy_mem.perm_of_res (resource_at (JTP.getThreadR Htid) (b, ofs)) = ((DTP.getThreadR (mtch_cnt Htid)) !! b) ofs ),
+      match_st js ds.
+  
+  (*match axioms*)
+  Lemma MTCH_ctn: forall {js tid ds},
+           match_st js ds ->
+           JTP.containsThread js tid -> DTP.containsThread ds tid.
+  Proof. intros ? ? ? MTCH. inversion MTCH. apply mtch_cnt. Qed.
+  Lemma MTCH_ctn': forall {js tid ds},
+           match_st js ds ->
+           DTP.containsThread ds tid -> JTP.containsThread js tid.
+  Proof. intros ? ? ? MTCH. inversion MTCH. apply mtch_cnt'. Qed.
+
+
+  Lemma ctn_irr: forall tid ds (cnt1 cnt2: DTP.containsThread ds tid),
+      DTP.getThreadC cnt1 = DTP.getThreadC cnt2.
+  Proof. intros.
+         
+         unfold DTP.getThreadC.
+         destruct ds; simpl.
+         f_equal; f_equal.
+         eapply proof_irrelevance.
+  Qed.
+
+  Lemma MTCH_getThreadC: forall js ds tid c,
+      forall (ctn: JTP.containsThread js tid)
+        (M: match_st js ds),
+        JTP.getThreadC ctn =  c ->
+        DTP.getThreadC (MTCH_ctn M ctn) =  c.
+  Proof. intros ? ? ? ? ? MTCH; inversion MTCH; subst.
+         intros HH; rewrite <- HH.
+         rewrite mtch_gtc.
+         apply ctn_irr.
+  Qed.
+       
+  Lemma MTCH_compat: forall js ds m,
+      match_st js ds ->
+      JSEM.mem_compatible js m ->
+      DSEM.mem_compatible ds m.
+  Proof. 
+    intros ? ? ? MTCH mc;
+    inversion MTCH; inversion mc; subst.
+    constructor.
+    - unfold DSEM.perm_compatible. intros tid cnt.
+      unfold permissions.permMapLt; intros b ofs.
+      eapply po_trans.
+      specialize (perm_comp tid (mtch_cnt' _ cnt)).
+      inversion perm_comp.
+      specialize (acc_coh (b, ofs)).
+      rewrite permissions.getMaxPerm_correct.
+      apply acc_coh.
+
+      
+      
+      rewrite <- permissions.restrPermMap_max.
+      specialize (acc_coh b).
+      
+      unfold max_accDess_cohere in max_coh.
+      
+      
+    Lemma MTCH_updt:
+      forall js ds tid c
+        (H0:match_st js ds)  (ctn: JTP.containsThread js tid),
+        match_st (JTP.updThreadC ctn c)
+                 (DTP.updThreadC (MTCH_ctn H0 ctn) c).
+          
+
+  (*Lemma parch_match: forall (js: jstate) (ds: dstate),
+      match_st js ds <-> ds = parch_state js.*)
+
+       (*
+  (*Init diagram*)
+  Lemma match_init: forall c, match_st (JSEM.initial_machine c) (DSEM.initial_machine c).
+
+  (*Core Diagram*)
+  Lemma parched_diagram: forall genv U U' m m' jst jst' ds ds',  
+      corestep JMachineSem genv (U, jst) m (U', jst') m' ->
+      match_st jst ds -> match_st jst ds -> 
+      corestep DMachineSem genv (U, ds)  m (U', ds') m'.
+        *)
+
+       
+  Variable genv: G.
+  Variable main: Values.val.
+  Lemma init_diagram:
+    forall (j : Values.Val.meminj) (U:schedule) (js : jstate)
+     (vals : list Values.val) (m : M),
+   initial_core JMachineSem genv main vals = Some (U, js) ->
+   exists (mu : SM_Injection) (ds : dstate),
+     as_inj mu = j /\
+     initial_core DMachineSem genv main vals = Some (U, ds) /\
+     DSEM.invariant ds /\
+     match_st js ds.
+
+  Lemma core_diagram:
+    forall (m : M)  (U U': schedule) 
+     (ds : dstate) (js js': jstate) 
+     (m' : M),
+   corestep JMachineSem genv (U, js) m (U', js') m' ->
+   match_st js ds ->
+   DSEM.invariant ds ->
+   exists (ds' : dstate) (mu' : SM_Injection),
+     DSEM.invariant ds' /\
+     match_st js' ds' /\
+     corestep DMachineSem genv (U, ds) m (U', ds') m'.
+
+  Lemma halted_diagram:
+    forall c, halted JMachineSem c = None.
+  
+
+
+
+
+
+
+
+
+
+
+ (* HERE ENDS THE NEW PART *)
   
  Definition perm_of_res (r: compcert_rmaps.RML.R.resource): shares.share. (*This must exists somwehre*)
  Admitted.
@@ -46,9 +195,7 @@ Module ClightErasure (SCH: Scheduler NatTID)(SEM: Semantics)<:Parching SCH SEM.
       eapply (Maps.PTree.map f TREE).
   Defined.
 
-  Definition pos_eq_nat_eq {p q: pos.pos} (pos_eq: p = q):(pos.n p = pos.n q).  rewrite pos_eq; reflexivity. Defined.
-  Definition size_change {cT js ds} (size_eq: juicy_machine.ThreadPool.num_threads(cT:=cT) js = compcert_threads.ThreadPool.num_threads(cT:=cT) ds) tid:=
-    fintype.cast_ord (pos_eq_nat_eq size_eq) tid.
+  
     
   Inductive match_st : jstate ->  dstate -> Prop:=
     MATCH_ST: forall (js:jstate) ds
